### Ambiguity

#### Ambiguous
```
E -> E + E | E * E | (E) | a
```
#### Unambiuous
```
E -> E + T | T
T -> T * F | F
F -> (E) | a
```
- The Unambiguus grammar is derived for the ambiguous one using information **not** specified in in the ambiguous grammar.
	- The operator "*" binds tighter than the operator "+".
	- Both the operators "*" and "+" are left associative.
	- Without the external information there is no way to make the transformation.
- With this information we can tell that:
``` a * a + b * b ```
is grouped as
``` (a * a) + (b * b) ```
rather than
``` a * ((a + b) * b) ```
